BusyLean/BusyLean.lean
@@ -4,3 +4,4 @@ import BusyLean.Parser
 import BusyLean.RunLemmas
 import BusyLean.Notation
 import BusyLean.Tactics
+import BusyLean.Nonhalt
